Inserters/ManyIdent.dfy
@@ -1,0 +1,75 @@
+module Inserters_ManyIdent {
+
+  import opened Circ
+  import opened ConservedSubcircuit
+  import opened MapFunction
+  import opened Inserters_Unary
+  import opened Modifiers.SwitchUF
+  import opened Modifiers_ManyParallel
+  import opened Inserters.Ident
+
+  opaque function ManyIdentUF(n: nat): (r: UpdateFunction)
+    ensures r.Valid()
+    ensures r.input_width == n
+    ensures r.output_width == n
+    ensures r.state_width == 0
+  {
+    reveal UpdateFunction.Valid();
+    UpdateFunction(
+      n, n, 0,
+      (si: SI) requires |si.inputs| == n && |si.state| == 0 =>
+        SO(si.inputs, [])
+      )
+  }
+
+  function ManyIdentInserterImpl(n: nat): (z: ScufInserter)
+    ensures z.Valid()
+  {
+    var z_ident := IdentInserter();
+    var z := ManyParallelInserter(z_ident, n);
+    z
+  }
+
+  lemma ManyIdentUFEquivInternal(n: nat, si: SI)
+    requires |si.inputs| == n
+    requires |si.state| == 0
+    ensures
+      && ManyParallelSF(IdentUF(), n, si) == SO(si.inputs, [])
+  {
+    reveal UpdateFunction.Valid();
+    reveal IdentUF();
+  }
+
+  lemma ManyIdentUFEquiv(n: nat)
+    ensures
+      var uf_base := ManyParallelUpdateFunction(IdentUF(), n);
+      var new_uf := ManyIdentUF(n);
+      UpdateFunctionsEquiv(new_uf, uf_base)
+  {
+    reveal IdentUF();
+    var uf_base := ManyParallelUpdateFunction(IdentUF(), n);
+    var new_uf := ManyIdentUF(n);
+    reveal UpdateFunction.Valid();
+    forall si | new_uf.SIVal(si)
+      ensures new_uf.sf(si) == uf_base.sf(si)
+    {
+      reveal ManyIdentUF();
+      reveal IdentUF();
+      reveal ManyParallelUpdateFunction();
+      ManyIdentUFEquivInternal(n, si);
+    }
+    reveal UpdateFunctionsEquiv();
+  }
+
+  opaque function ManyIdentInserter(n: nat): (z: ScufInserter)
+    ensures z.Valid()
+    ensures z.uf == ManyIdentUF(n)
+  {
+    var z_base := ManyIdentInserterImpl(n);
+    var new_uf := ManyIdentUF(n);
+    ManyIdentUFEquiv(n);
+    var z := SwitchUFModifier(z_base, new_uf);
+    z
+  }
+
+}
