Inserters/Mux2.dfy
@@ -1,0 +1,305 @@
+module Inserters_Mux2 {
+
+  import Std.Collections.Seq
+
+  import opened ConservedSubcircuit
+  import opened Inserters.Ident
+  import opened Inserters_ManyIdent
+  import opened Inserters.Inv
+  import opened Inserters.And
+  import opened Inserters.Or
+  import opened SelfConnect
+  import opened MapFunction
+  import opened Modifiers.Merge
+  import opened Modifiers_Series
+  import opened Modifiers_ForwardConnect
+  import opened Modifiers.NewOutputs
+  import opened Modifiers.SwitchUF
+
+  opaque function Mux2UF(): (uf: UpdateFunction)
+    ensures uf.Valid()
+    ensures uf.input_width == 3
+    ensures uf.output_width == 1
+    ensures uf.state_width == 0
+  {
+    reveal UpdateFunction.Valid();
+    UpdateFunction(
+      3, 1, 0,
+      (si: SI) requires |si.inputs| == 3 && |si.state| == 0 =>
+        SO([if si.inputs[0] then si.inputs[2] else si.inputs[1]], []))
+  }
+
+  function GetNewOutputs(): (new_outputs: seq<nat>)
+    ensures NewOutputsValid(4, new_outputs)
+  {
+    var new_outputs := [0, 3, 1, 2];
+    assert NewOutputsValid(4, new_outputs) by {
+      reveal NewOutputsValid();
+      reveal Seq.HasNoDuplicates();
+    }
+    new_outputs
+  }
+
+  opaque function Mux2UFBase(): (uf: UpdateFunction)
+    ensures uf.Valid()
+    ensures uf.input_width == 3
+    ensures uf.output_width == 1
+    ensures uf.state_width == 0
+  {
+    var uf_sel := IdentUF();
+    var uf_notsel := InvUF();
+    var conn := Mux2IdentInvForwardConn();
+    var uf_sel_notsel := ForwardConnectUF(uf_sel, uf_notsel, conn);
+    assert uf_sel_notsel.input_width == 1;
+    assert uf_sel_notsel.output_width == 2;
+    assert uf_sel_notsel.state_width == 0;
+
+    // Create a module that just bundles the 'A' and 'B' input signals together
+    var uf_a_b := ManyIdentUF(2);
+    assert uf_a_b.input_width == 2;
+    assert uf_a_b.output_width == 2;
+    assert uf_a_b.state_width == 0;
+
+    // Now join those two modules.
+    var uf_sel_notsel_a_b := MergeUpdateFunctions(uf_sel_notsel, uf_a_b);
+    assert uf_sel_notsel_a_b.input_width == 3;
+    assert uf_sel_notsel_a_b.output_width == 4;
+    assert uf_sel_notsel_a_b.state_width == 0;
+
+    // Rearrange the output wires so that we can feed them easily into the and gates.
+    var new_outputs := GetNewOutputs();
+
+    var uf_sel_a_notsel_b := NewOutputsUpdateFunction(uf_sel_notsel_a_b, new_outputs);
+    assert uf_sel_a_notsel_b.input_width == 3;
+    assert uf_sel_a_notsel_b.output_width == 4;
+    assert uf_sel_a_notsel_b.state_width == 0;
+
+    // Now build a module with two and gates in parallel
+    var uf_ands := MergeUpdateFunctions(AndUF(), AndUF());
+    assert uf_ands.input_width == 4;
+    assert uf_ands.output_width == 2;
+    assert uf_ands.state_width == 0;
+    
+    // And feed the other module into the and gates.
+    var uf_upto_ands := SeriesUpdateFunction(uf_sel_a_notsel_b, uf_ands);
+    assert uf_upto_ands.input_width == 3;
+    assert uf_upto_ands.output_width == 2;
+    assert uf_upto_ands.state_width == 0;
+
+    // And finally feed the outputs of the ands into an or.
+    var uf_mux := SeriesUpdateFunction(uf_upto_ands, OrUF());
+    assert uf_mux.input_width == 3;
+    assert uf_mux.output_width == 1;
+    assert uf_mux.state_width == 0;
+    uf_mux
+  }
+
+  lemma {:vcs_split_on_every_assert} Mux2UFEquiv()
+    // FixMe: Using 29M
+    ensures UpdateFunctionsEquiv(Mux2UF(), Mux2UFBase())
+  {
+    var uf := Mux2UF();
+    var uf_base := Mux2UFBase();
+    assert uf.input_width == uf_base.input_width;
+    assert uf.output_width == uf_base.output_width;
+    assert uf.state_width == uf_base.state_width;
+    forall si: SI | uf.SIVal(si)
+      ensures
+        && uf.sf.requires(si)
+        && uf_base.sf.requires(si)
+        && (uf.sf(si) == uf_base.sf(si))
+    {
+      // Proving behavior for (ident inv)
+      var uf_sel := IdentUF();
+      var uf_notsel := InvUF();
+      var conn := Mux2IdentInvForwardConn();
+      var uf_sel_notsel := ForwardConnectUF(uf_sel, uf_notsel, conn);
+      var si_sel_notsel := SI([si.inputs[0]], []);
+      assert uf_sel_notsel.input_width == 1;
+      reveal UpdateFunction.Valid();
+      var so_sel_notsel := uf_sel_notsel.sf(si_sel_notsel);
+      assert so_sel_notsel.outputs == [si.inputs[0], !si.inputs[0]] by {
+        var si_sel := SI([si.inputs[0]], []);
+        var so_sel := uf_sel.sf(si_sel);
+        assert so_sel == SO([si.inputs[0]], []) by {
+          reveal IdentUF();
+        }
+        var si_inv_input := conn.NIO2I([], so_sel.outputs);
+        assert si_inv_input == [so_sel.outputs[0]] by {
+          reveal Mux2IdentInvForwardConn();
+        }
+        var si_inv := SI(si_inv_input, []);
+        var so_inv := uf_notsel.sf(si_inv);
+        assert so_inv == SO([!si.inputs[0]], []) by {
+          reveal InvUF();
+        }
+        reveal ForwardConnectUF();
+        assert so_sel_notsel == ForwardConnectSF(uf_sel, uf_notsel, conn, si_sel_notsel);
+        assert so_sel_notsel == SO(so_sel.outputs + so_inv.outputs, so_sel.state + so_inv.state) by {
+          var uf1 := uf_sel;
+          var uf2 := uf_notsel;
+          var si1: SI := SI(si_sel_notsel.inputs[..uf1.input_width], si_sel_notsel.state[..uf1.state_width]);
+          assert si1 == si_sel;
+          var so1 := uf1.sf(si1);
+          var si2_true_input := si_sel_notsel.inputs[uf1.input_width..];
+          var si2_input := conn.NIO2I(si2_true_input, so1.outputs);
+          var si2 := SI(si2_input, si_sel_notsel.state[uf1.state_width..]);
+          assert si2 == si_inv;
+          var so2 := uf2.sf(si2);
+          var so := SO(so1.outputs + so2.outputs, so1.state + so2.state);
+        }
+      }
+      // Proving behavior for after we add the idents in and rearrange.
+      // Create a module that just bundles the 'A' and 'B' input signals together
+      var uf_a_b := ManyIdentUF(2);
+      var si_a_b := SI(si.inputs[1..], []);
+
+      // Now join those two modules.
+      var uf_sel_notsel_a_b := MergeUpdateFunctions(uf_sel_notsel, uf_a_b);
+      var so_sel_notsel_a_b := uf_sel_notsel_a_b.sf(si);
+      assert so_sel_notsel_a_b == SO([si.inputs[0], !si.inputs[0], si.inputs[1], si.inputs[2]], []) by {
+        MergeUpdateFunctionBehav(uf_sel_notsel, uf_a_b, si);
+        assert uf_sel_notsel.sf(SI([si.inputs[0]], [])) == SO([si.inputs[0], !si.inputs[0]], []);
+        reveal ManyIdentUF();
+        assert uf_a_b.sf(SI(si.inputs[1..], [])) == SO(si.inputs[1..], []);
+        assert MergeSF(uf_sel_notsel, uf_a_b, si) == SO([si.inputs[0], !si.inputs[0], si.inputs[1], si.inputs[2]], []) by {
+          var uf1 := uf_sel_notsel;
+          var uf2 := uf_a_b;
+          var si1 := SI(si.inputs[..uf1.input_width], si.state[..uf1.state_width]);
+          var si2 := SI(si.inputs[uf1.input_width..], si.state[uf1.state_width..]);
+          assert si1 == si_sel_notsel;
+          assert si2 == si_a_b;
+          reveal UpdateFunction.Valid();
+          var so1 := uf1.sf(si1);
+          var so2 := uf2.sf(si2);
+          var so := SO(so1.outputs + so2.outputs, so1.state + so2.state);
+        }
+      }
+      // Rearrange the output wires so that we can feed them easily into the and gates.
+      var new_outputs := GetNewOutputs();
+      var uf_sel_a_notsel_b := NewOutputsUpdateFunction(uf_sel_notsel_a_b, new_outputs);
+
+      var so_sel_a_notsel_b := uf_sel_a_notsel_b.sf(si);
+      assert so_sel_a_notsel_b == SO([si.inputs[0], si.inputs[2], !si.inputs[0], si.inputs[1]], []) by {
+        reveal NewOutputsUpdateFunction();
+      }
+
+      // Now build a module with two and gates in parallel
+      var uf_ands := MergeUpdateFunctions(AndUF(), AndUF());
+      
+      // And feed the other module into the and gates.
+      var uf_upto_ands := SeriesUpdateFunction(uf_sel_a_notsel_b, uf_ands);
+      var so_upto_ands := uf_upto_ands.sf(si);
+      assert so_upto_ands == SO([si.inputs[0] && si.inputs[2], (!si.inputs[0]) && si.inputs[1]], []) by {
+        reveal AndUF();
+        var si_ands := SI(so_sel_a_notsel_b.outputs, []);
+        MergeUpdateFunctionBehav(AndUF(), AndUF(), si_ands);
+        var uf1 := AndUF();
+        var uf2 := AndUF();
+        var si1 := SI(si_ands.inputs[..uf1.input_width], si_ands.state[..uf1.state_width]);
+        var si2 := SI(si_ands.inputs[uf1.input_width..], si_ands.state[uf1.state_width..]);
+        assert si1 == SI([si.inputs[0], si.inputs[2]], []);
+        assert si2 == SI([!si.inputs[0], si.inputs[1]], []);
+        reveal UpdateFunction.Valid();
+        var so1 := uf1.sf(si1);
+        var so2 := uf2.sf(si2);
+        var so := SO(so1.outputs + so2.outputs, so1.state + so2.state);
+        reveal SeriesUpdateFunction();
+      }
+
+      // And finally feed the outputs of the ands into an or.
+      var uf_mux := SeriesUpdateFunction(uf_upto_ands, OrUF());
+
+      assert uf.sf(si) == uf_mux.sf(si) by {
+        reveal OrUF();
+        reveal SeriesUpdateFunction();
+        var si_or := SI(so_upto_ands.outputs, []);
+        var so_or := OrUF().sf(si_or);
+        assert so_or == SO([(si.inputs[0] && si.inputs[2]) || ((!si.inputs[0]) && si.inputs[1])], []);
+        var so_mux := uf_mux.sf(si);
+        assert so_mux == SO([(si.inputs[0] && si.inputs[2]) || ((!si.inputs[0]) && si.inputs[1])], []);
+        reveal Mux2UF();
+      }
+      assert uf_base == uf_mux by {
+        reveal Mux2UFBase();
+      }
+    }
+    reveal UpdateFunctionsEquiv();
+  }
+
+  // A mux consists of
+  // Three inputs (sel, A, B)
+  // inv_sel = ! sel
+  // A_sel   = A && inv_sel
+  // B_sel   = B && sel
+  // result  = A_sel || B_sel
+  
+  opaque function Mux2IdentInvForwardConn(): (r: InternalConnection)
+    // Takes the output from ident and feeds it into a inv
+    ensures r.Valid()
+    ensures r.i_width == 1
+    ensures r.ni_width == 0
+    ensures r.o_width == 1
+  {
+    var ni_width := 0;
+    var i_width := 1;
+    var o_width := 1;
+    var connections := map[0 := 0];
+    var i2ni := [];
+    var nio2i := [(true, 0)];
+    var conn := InternalConnection(ni_width, i_width, o_width, connections, i2ni, nio2i);
+    assert conn.Valid() by {
+      reveal InternalConnection.ConnectionsValid();
+      reveal InternalConnection.ToNIMapValid();
+      reveal InternalConnection.ToIMapValid();
+      reveal Seq.HasNoDuplicates();
+    }
+    conn
+  }
+
+  function Mux2InserterImpl(): (z: ScufInserter)
+    ensures z.Valid()
+    ensures z.uf == Mux2UFBase()
+  {
+    // Create a module that takes in the 'sel' signal and outputs the 'sel' and !'sel'.
+    var z_sel := IdentInserter();
+    var z_notsel := InvInserter();
+    var conn := Mux2IdentInvForwardConn();
+    var z_sel_notsel := ForwardConnectionModifier(z_sel, z_notsel, conn);
+
+    // Create a module that just bundles the 'A' and 'B' input signals together
+    var z_a_b := ManyIdentInserter(2);
+
+    // Now join those two modules.
+    var z_sel_notsel_a_b := MergeModifier(z_sel_notsel, z_a_b);
+
+    // Rearrange the output wires so that we can feed them easily into the and gates.
+    var new_outputs := GetNewOutputs();
+    var z_sel_a_notsel_b := NewOutputsModifier(z_sel_notsel_a_b, new_outputs);
+
+    // Now build a module with two and gates in parallel
+    var z_ands := MergeModifier(AndInserter(), AndInserter());
+    
+    // And feed the other module into the and gates.
+    var z_upto_ands := SeriesModifier(z_sel_a_notsel_b, z_ands);
+
+    // And finally feed the outputs of the ands into an or.
+    var z_mux := SeriesModifier(z_upto_ands, OrInserter());
+    assert z_mux.uf == Mux2UFBase() by {
+      reveal Mux2UFBase();
+    }
+    z_mux
+  }
+
+  function Mux2Inserter(): (z: ScufInserter)
+    ensures z.Valid()
+    ensures z.uf == Mux2UF()
+  {
+    var z_base := Mux2InserterImpl();
+    var new_uf := Mux2UF();
+    Mux2UFEquiv();
+    assert UpdateFunctionsEquiv(new_uf, Mux2UFBase());
+    var z := SwitchUFModifier(z_base, new_uf);
+    z
+  }
+}
